examples/nsl_pk/DY.Example.NSL.Protocol.Stateful.fst
@@ -79,8 +79,8 @@ let send_msg1 global_sess_id alice sess_id =
   let*? st = get_state alice sess_id in
   guard_tr (InitiatorSentMsg1? st);*?
   let InitiatorSentMsg1 bob n_a = st in
-  let*? pk_b = get_public_key alice global_sess_id.pki (LongTermPkEncKey "NSL.PublicKey") bob in
-  let* nonce = mk_rand PkNonce (long_term_key_label alice) 32 in
+  let*? pk_b = get_public_key alice global_sess_id.pki (LongTermPkeKey "NSL.PublicKey") bob in
+  let* nonce = mk_rand PkeNonce (long_term_key_label alice) 32 in
   let msg = compute_message1 alice bob pk_b n_a nonce in
   let* msg_id = send_msg msg in
   return (Some msg_id)
@@ -88,7 +88,7 @@ let send_msg1 global_sess_id alice sess_id =
 val prepare_msg2: nsl_global_sess_ids -> principal -> timestamp -> traceful (option state_id)
 let prepare_msg2 global_sess_id bob msg_id =
   let*? msg = recv_msg msg_id in
-  let*? sk_b = get_private_key bob global_sess_id.private_keys (LongTermPkEncKey "NSL.PublicKey") in
+  let*? sk_b = get_private_key bob global_sess_id.private_keys (LongTermPkeKey "NSL.PublicKey") in
   let*? msg1: message1 = return (decode_message1 bob msg sk_b) in
   let* n_b = mk_rand NoUsage (nsl_nonce_label msg1.alice bob) 32 in
   trigger_event bob (Respond1 msg1.alice bob msg1.n_a n_b);*
@@ -101,8 +101,8 @@ let send_msg2 global_sess_id bob sess_id =
   let*? st = get_state bob sess_id in
   guard_tr (ResponderSentMsg2? st);*?
   let ResponderSentMsg2 alice n_a n_b = st in
-  let*? pk_a = get_public_key bob global_sess_id.pki (LongTermPkEncKey "NSL.PublicKey") alice in
-  let* nonce = mk_rand PkNonce (long_term_key_label bob) 32 in
+  let*? pk_a = get_public_key bob global_sess_id.pki (LongTermPkeKey "NSL.PublicKey") alice in
+  let* nonce = mk_rand PkeNonce (long_term_key_label bob) 32 in
   let msg = compute_message2 bob {n_a; alice;} pk_a n_b nonce in
   let* msg_id = send_msg msg in
   return (Some msg_id)
@@ -110,7 +110,7 @@ let send_msg2 global_sess_id bob sess_id =
 val prepare_msg3: nsl_global_sess_ids -> principal -> state_id -> timestamp -> traceful (option unit)
 let prepare_msg3 global_sess_id alice sess_id msg_id =
   let*? msg = recv_msg msg_id in
-  let*? sk_a = get_private_key alice global_sess_id.private_keys (LongTermPkEncKey "NSL.PublicKey") in
+  let*? sk_a = get_private_key alice global_sess_id.private_keys (LongTermPkeKey "NSL.PublicKey") in
   let*? st = get_state alice sess_id in
   guard_tr (InitiatorSentMsg1? st);*?
   let InitiatorSentMsg1 bob n_a = st in
@@ -124,8 +124,8 @@ let send_msg3 global_sess_id alice sess_id =
   let*? st = get_state alice sess_id in
   guard_tr (InitiatorSentMsg3? st);*?
   let InitiatorSentMsg3 bob n_a n_b = st in
-  let*? pk_b = get_public_key alice global_sess_id.pki (LongTermPkEncKey "NSL.PublicKey") bob in
-  let* nonce = mk_rand PkNonce (long_term_key_label alice) 32 in
+  let*? pk_b = get_public_key alice global_sess_id.pki (LongTermPkeKey "NSL.PublicKey") bob in
+  let* nonce = mk_rand PkeNonce (long_term_key_label alice) 32 in
   let msg = compute_message3 alice bob pk_b n_b nonce in
   let* msg_id = send_msg msg in
   return (Some msg_id)
@@ -133,7 +133,7 @@ let send_msg3 global_sess_id alice sess_id =
 val prepare_msg4: nsl_global_sess_ids -> principal -> state_id -> timestamp -> traceful (option unit)
 let prepare_msg4 global_sess_id bob sess_id msg_id =
   let*? msg = recv_msg msg_id in
-  let*? sk_b = get_private_key bob global_sess_id.private_keys (LongTermPkEncKey "NSL.PublicKey") in
+  let*? sk_b = get_private_key bob global_sess_id.private_keys (LongTermPkeKey "NSL.PublicKey") in
   let*? st = get_state bob sess_id in
   guard_tr (ResponderSentMsg2? st);*?
   let ResponderSentMsg2 alice n_a n_b = st in
