examples/nsl_pk/DY.Example.NSL.Protocol.Total.Proof.fst
@@ -23,7 +23,7 @@ let crypto_predicates_nsl = {
 
   pkenc_pred = {
     pred = (fun tr sk_usage msg ->
-      (exists prin. sk_usage == long_term_key_type_to_usage (LongTermPkEncKey "NSL.PublicKey") prin /\ (
+      (exists prin. sk_usage == long_term_key_type_to_usage (LongTermPkeKey "NSL.PublicKey") prin /\ (
         match parse message msg with
         | Some (Msg1 msg1) -> (
           let (alice, bob) = (msg1.alice, prin) in
@@ -70,9 +70,9 @@ val compute_message1_proof:
     // From random generation
     is_secret (long_term_key_label alice) tr nonce /\
     // From random generation
-    nonce `has_usage tr` PkNonce /\
+    nonce `has_usage tr` PkeNonce /\
     // From PKI invariants
-    is_public_key_for tr pk_b (LongTermPkEncKey "NSL.PublicKey") bob
+    is_public_key_for tr pk_b (LongTermPkeKey "NSL.PublicKey") bob
   )
   (ensures is_publishable tr (compute_message1 alice bob pk_b n_a nonce))
 let compute_message1_proof tr alice bob pk_b n_a nonce =
@@ -92,7 +92,7 @@ val decode_message1_proof:
   Lemma
   (requires
     // From PrivateKeys invariants
-    is_private_key_for tr sk_b (LongTermPkEncKey "NSL.PublicKey") bob /\
+    is_private_key_for tr sk_b (LongTermPkeKey "NSL.PublicKey") bob /\
     // From the network
     bytes_invariant tr msg_cipher
   )
@@ -126,9 +126,9 @@ val compute_message2_proof:
     // From the random generation
     is_secret (long_term_key_label bob) tr nonce /\
     // From the random generation
-    nonce `has_usage tr` PkNonce /\
+    nonce `has_usage tr` PkeNonce /\
     // From the PKI
-    is_public_key_for tr pk_a (LongTermPkEncKey "NSL.PublicKey") msg1.alice
+    is_public_key_for tr pk_a (LongTermPkeKey "NSL.PublicKey") msg1.alice
   )
   (ensures
     is_publishable tr (compute_message2 bob msg1 pk_a n_b nonce)
@@ -151,7 +151,7 @@ val decode_message2_proof:
     // From the NSL state invariant
     is_secret (nsl_nonce_label alice bob) tr n_a /\
     // From the PrivateKeys invariant
-    is_private_key_for tr sk_a (LongTermPkEncKey "NSL.PublicKey") alice /\
+    is_private_key_for tr sk_a (LongTermPkeKey "NSL.PublicKey") alice /\
     // From the network
     bytes_invariant tr msg_cipher
   )
@@ -188,9 +188,9 @@ val compute_message3_proof:
     // From the random generation
     is_secret (long_term_key_label alice) tr nonce /\
     // From the random generation
-    nonce `has_usage tr` PkNonce /\
+    nonce `has_usage tr` PkeNonce /\
     // From the PKI
-    is_public_key_for tr pk_b (LongTermPkEncKey "NSL.PublicKey") bob
+    is_public_key_for tr pk_b (LongTermPkeKey "NSL.PublicKey") bob
   )
   (ensures
     is_publishable tr (compute_message3 alice bob pk_b n_b nonce)
@@ -215,7 +215,7 @@ val decode_message3_proof:
     // From the NSL state invariant
     get_label tr n_b == nsl_nonce_label alice bob /\
     // From the PrivateKeys invariant
-    is_private_key_for tr sk_b (LongTermPkEncKey "NSL.PublicKey") bob /\
+    is_private_key_for tr sk_b (LongTermPkeKey "NSL.PublicKey") bob /\
     // From the network
     bytes_invariant tr msg_cipher
   )
